Manually merge TLS.Curve25519.fst from quic2c

src/tls/TLS.Curve25519.fst
@@ -2,11 +2,8 @@ module TLS.Curve25519
 
 open FStar.Bytes
 open FStar.Error
-open Mem
 
-module X = Hacl.Curve25519
-module CC = CoreCrypto
-module U32 = FStar.UInt32
+open FStar.HyperStack.ST
 
 type scalar = lbytes 32
 type point = lbytes 32
@@ -17,7 +14,7 @@ let pubshare (k:keyshare) : Tot point = fst k
 //NS: 2/2 See issue #21 and #14
 // Test files replace the rand function with a deterministic variant.
 // let rand: ref (n:nat -> ST (lbytes n) (requires fun h->True) (ensures fun h0 _ h1 -> modifies_none h0 h1)) =
-//   ralloc root CC.random
+//   ralloc root CoreCrypto.random
 
 let scalarmult (secret:Bytes.lbytes 32) (point:Bytes.lbytes 32)
   : ST (lbytes 32)
@@ -29,8 +26,11 @@ let keygen () : ST keyshare
   (requires (fun h0 -> True))
   (ensures (fun h0 _ h1 -> modifies_none h0 h1))
   =
-  let s : lbytes 32 = CC.random 32 in
-  let base_point = Bytes.set_byte (Bytes.create 32ul 0uy) 0ul 9uy in
+  let s : lbytes 32 = CoreCrypto.random 32 in
+  let base_point =
+    Bytes.bytes_of_hex
+      "0900000000000000000000000000000000000000000000000000000000000000" in
+  assume (Bytes.length base_point == 32);
   scalarmult s base_point, s
 
 let mul (k:scalar) (p:point) : ST point
